Charge!/src/Charge/Tactics/Views/EmbedView.v
@@ -49,7 +49,7 @@ Section EmbedFuncInst.
   Definition embed_opsOk (es : embed_ops) : Prop :=
     forall t t',
       match is t , is t' , es t t' return Prop with
-        | Some a , Some b , Some T => @Embed _ a _ _ T
+        | _Some a , _Some b , Some T => @Embed _ a _ _ T
         | _ , _ , _ => True
       end.
 
